Started fixing Hoare logic

utp_hoare.thy
@@ -4,128 +4,127 @@ begin
 
 text \<open>Hoare triples\<close>
 
-definition hoare_r :: "('s \<Rightarrow> bool) \<Rightarrow> 's rel \<Rightarrow> ('s \<Rightarrow> bool) \<Rightarrow> bool" where
-[rel]: "hoare_r p Q r = ((p\<^sup>< \<longrightarrow> r\<^sup>>)\<^sub>u \<sqsubseteq> Q)"
+definition hoare_r :: "('s \<Rightarrow> bool) \<Rightarrow> 's hrel \<Rightarrow> ('s \<Rightarrow> bool) \<Rightarrow> bool" where
+[pred]: "hoare_r p Q r = ((p\<^sup>< \<longrightarrow> r\<^sup>>)\<^sub>e \<sqsubseteq> Q)"
 
-syntax "_hoare_r" :: "logic \<Rightarrow> logic \<Rightarrow> logic \<Rightarrow> logic" ("\<^bold>{_\<^bold>}/ _/ \<^bold>{_\<^bold>}")
+syntax 
+  "_hoare_r" :: "logic \<Rightarrow> logic \<Rightarrow> logic \<Rightarrow> logic" ("\<^bold>{_\<^bold>}/ _/ \<^bold>{_\<^bold>}")
+  "_hoare_r" :: "logic \<Rightarrow> logic \<Rightarrow> logic \<Rightarrow> logic" ("H{_}/ _/ {_}")
+
 translations "_hoare_r P S Q" == "CONST hoare_r (P)\<^sub>e S (Q)\<^sub>e"
+
 
 named_theorems hoare and hoare_safe
 
-thm relcomp_unfold Id_on_iff
+lemma hoare_meaning: "H{p}Q{r} = (\<forall> s s'. p s \<and> Q (s, s') \<longrightarrow> r s')"
+  by (pred_auto)
 
-lemma relcomp_iff: "(a, b) \<in> P O Q \<longleftrightarrow> (\<exists> c. (a, c) \<in> P \<and> (c, b) \<in> Q)"
-  by (simp add: relcomp_unfold)
+lemma hoare_alt_def: "\<^bold>{b\<^bold>}P\<^bold>{c\<^bold>} = (P ;; \<questiondown>c? \<sqsubseteq> \<questiondown>b? ;; P)"
+  by (pred_auto)
 
-lemma hoare_meaning: "\<^bold>{p\<^bold>}Q\<^bold>{r\<^bold>} = (\<forall> s s'. p s \<and> (s, s') \<in> Q \<longrightarrow> r s')"
-  by (rel_auto)
+lemma hoare_assume: "\<^bold>{P\<^bold>}S\<^bold>{Q\<^bold>} \<Longrightarrow> \<questiondown>P? ;; S = \<questiondown>P? ;; S ;; \<questiondown>Q?"
+  by (pred_auto)
 
-lemma hoare_alt_def: "\<^bold>{b\<^bold>}P\<^bold>{c\<^bold>} = (P \<Zcomp> \<questiondown>c? \<sqsubseteq> \<questiondown>b? \<Zcomp> P)"
-  by (rel_auto)
+lemma hoare_pre_assume_1: "\<^bold>{b \<and> c\<^bold>}P\<^bold>{d\<^bold>} = \<^bold>{c\<^bold>}\<questiondown>b? ;; P\<^bold>{d\<^bold>}"
+  by (pred_auto)
 
-lemma hoare_assume: "\<^bold>{P\<^bold>}S\<^bold>{Q\<^bold>} \<Longrightarrow> \<questiondown>P? \<Zcomp> S = \<questiondown>P? \<Zcomp> S \<Zcomp> \<questiondown>Q?"
-  by (rel_auto)
-
-lemma hoare_pre_assume_1: "\<^bold>{b \<and> c\<^bold>}P\<^bold>{d\<^bold>} = \<^bold>{c\<^bold>}\<questiondown>b? \<Zcomp> P\<^bold>{d\<^bold>}"
-  by (rel_auto)
-
-lemma hoare_pre_assume_2: "\<^bold>{b \<and> c\<^bold>}P\<^bold>{d\<^bold>} = \<^bold>{b\<^bold>}\<questiondown>c? \<Zcomp> P\<^bold>{d\<^bold>}"
-  by rel_auto
+lemma hoare_pre_assume_2: "\<^bold>{b \<and> c\<^bold>}P\<^bold>{d\<^bold>} = \<^bold>{b\<^bold>}\<questiondown>c? ;; P\<^bold>{d\<^bold>}"
+  by pred_auto
                                
 lemma hoare_test [hoare_safe]: "`p \<and> b \<longrightarrow> q` \<Longrightarrow> \<^bold>{p\<^bold>}\<questiondown>b?\<^bold>{q\<^bold>}"
-  by rel_auto
+  by pred_auto
 
-lemma hoare_gcmd [hoare_safe]: "\<^bold>{p \<and> b\<^bold>}P\<^bold>{q\<^bold>} \<Longrightarrow> \<^bold>{p\<^bold>}\<questiondown>b? \<Zcomp> P\<^bold>{q\<^bold>}"
-  by rel_auto
+lemma hoare_gcmd [hoare_safe]: "\<^bold>{p \<and> b\<^bold>}P\<^bold>{q\<^bold>} \<Longrightarrow> \<^bold>{p\<^bold>}\<questiondown>b? ;; P\<^bold>{q\<^bold>}"
+  by pred_auto
 
 lemma hoare_r_conj [hoare_safe]: "\<lbrakk> \<^bold>{p\<^bold>}Q\<^bold>{r\<^bold>}; \<^bold>{p\<^bold>}Q\<^bold>{s\<^bold>} \<rbrakk> \<Longrightarrow> \<^bold>{p\<^bold>}Q\<^bold>{r \<and> s\<^bold>}"
-  by rel_auto
+  by pred_auto
 
 lemma hoare_r_weaken_pre [hoare]:
   "\<^bold>{p\<^bold>}Q\<^bold>{r\<^bold>} \<Longrightarrow> \<^bold>{p \<and> q\<^bold>}Q\<^bold>{r\<^bold>}"
   "\<^bold>{q\<^bold>}Q\<^bold>{r\<^bold>} \<Longrightarrow> \<^bold>{p \<and> q\<^bold>}Q\<^bold>{r\<^bold>}"
-  by rel_auto+
+  by pred_auto+
 
 lemma pre_str_hoare_r:
   assumes "`p\<^sub>1 \<longrightarrow> p\<^sub>2`" and "\<^bold>{p\<^sub>2\<^bold>}C\<^bold>{q\<^bold>}"
   shows "\<^bold>{p\<^sub>1\<^bold>}C\<^bold>{q\<^bold>}"
-  using assms by rel_auto
+  using assms by pred_auto
     
 lemma post_weak_hoare_r:
   assumes "\<^bold>{p\<^bold>}C\<^bold>{q\<^sub>2\<^bold>}" and "`q\<^sub>2 \<longrightarrow> q\<^sub>1`"
   shows "\<^bold>{p\<^bold>}C\<^bold>{q\<^sub>1\<^bold>}" 
-  using assms by rel_auto
+  using assms by pred_auto
 
 lemma hoare_r_conseq: "\<lbrakk> \<^bold>{p\<^sub>2\<^bold>}S\<^bold>{q\<^sub>2\<^bold>}; `p\<^sub>1 \<longrightarrow> p\<^sub>2`; `q\<^sub>2 \<longrightarrow> q\<^sub>1` \<rbrakk> \<Longrightarrow> \<^bold>{p\<^sub>1\<^bold>}S\<^bold>{q\<^sub>1\<^bold>}"
-  by rel_auto
+  by pred_auto
 
 lemma hoare_r_cut:
   assumes "\<^bold>{b\<^bold>}P\<^bold>{b\<^bold>}" "\<^bold>{b \<and> c\<^bold>}P\<^bold>{c\<^bold>}"
   shows "\<^bold>{b \<and> c\<^bold>}P\<^bold>{b \<and> c\<^bold>}"
-  using assms by rel_auto
+  using assms by pred_auto
 
 lemma hoare_r_cut_simple: 
   assumes "\<^bold>{b\<^bold>}P\<^bold>{b\<^bold>}" "\<^bold>{c\<^bold>}P\<^bold>{c\<^bold>}"
   shows "\<^bold>{b \<and> c\<^bold>}P\<^bold>{b \<and> c\<^bold>}"
-  using assms by rel_auto
+  using assms by pred_auto
 
 lemma hoare_oracle: "\<^bold>{p\<^bold>}false\<^bold>{q\<^bold>}"
   by (simp add: hoare_r_def)
 
 subsection \<open> Sequence Laws \<close>
 
-lemma seq_hoare_r: "\<lbrakk> \<^bold>{p\<^bold>}Q\<^sub>1\<^bold>{s\<^bold>} ; \<^bold>{s\<^bold>}Q\<^sub>2\<^bold>{r\<^bold>} \<rbrakk> \<Longrightarrow> \<^bold>{p\<^bold>}Q\<^sub>1 \<Zcomp> Q\<^sub>2\<^bold>{r\<^bold>}"
+lemma seq_hoare_r: "\<lbrakk> \<^bold>{p\<^bold>}Q\<^sub>1\<^bold>{s\<^bold>} ; \<^bold>{s\<^bold>}Q\<^sub>2\<^bold>{r\<^bold>} \<rbrakk> \<Longrightarrow> \<^bold>{p\<^bold>}Q\<^sub>1 ;; Q\<^sub>2\<^bold>{r\<^bold>}"
   by (rel_force)
  
-lemma seq_hoare_invariant [hoare_safe]: "\<lbrakk> \<^bold>{p\<^bold>}Q\<^sub>1\<^bold>{p\<^bold>} ; \<^bold>{p\<^bold>}Q\<^sub>2\<^bold>{p\<^bold>} \<rbrakk> \<Longrightarrow> \<^bold>{p\<^bold>}Q\<^sub>1 \<Zcomp> Q\<^sub>2\<^bold>{p\<^bold>}"
+lemma seq_hoare_invariant [hoare_safe]: "\<lbrakk> \<^bold>{p\<^bold>}Q\<^sub>1\<^bold>{p\<^bold>} ; \<^bold>{p\<^bold>}Q\<^sub>2\<^bold>{p\<^bold>} \<rbrakk> \<Longrightarrow> \<^bold>{p\<^bold>}Q\<^sub>1 ;; Q\<^sub>2\<^bold>{p\<^bold>}"
   by (rel_force)
 
 lemma seq_hoare_stronger_pre_1 [hoare_safe]: 
-  "\<lbrakk> \<^bold>{p \<and> q\<^bold>}Q\<^sub>1\<^bold>{p \<and> q\<^bold>} ; \<^bold>{p \<and> q\<^bold>}Q\<^sub>2\<^bold>{q\<^bold>} \<rbrakk> \<Longrightarrow> \<^bold>{p \<and> q\<^bold>}Q\<^sub>1 \<Zcomp> Q\<^sub>2\<^bold>{q\<^bold>}"
+  "\<lbrakk> \<^bold>{p \<and> q\<^bold>}Q\<^sub>1\<^bold>{p \<and> q\<^bold>} ; \<^bold>{p \<and> q\<^bold>}Q\<^sub>2\<^bold>{q\<^bold>} \<rbrakk> \<Longrightarrow> \<^bold>{p \<and> q\<^bold>}Q\<^sub>1 ;; Q\<^sub>2\<^bold>{q\<^bold>}"
   using seq_hoare_r by blast
 
 lemma seq_hoare_stronger_pre_2 [hoare_safe]: 
-  "\<lbrakk> \<^bold>{p \<and> q\<^bold>}Q\<^sub>1\<^bold>{p \<and> q\<^bold>} ; \<^bold>{p \<and> q\<^bold>}Q\<^sub>2\<^bold>{p\<^bold>} \<rbrakk> \<Longrightarrow> \<^bold>{p \<and> q\<^bold>}Q\<^sub>1 \<Zcomp> Q\<^sub>2\<^bold>{p\<^bold>}"
+  "\<lbrakk> \<^bold>{p \<and> q\<^bold>}Q\<^sub>1\<^bold>{p \<and> q\<^bold>} ; \<^bold>{p \<and> q\<^bold>}Q\<^sub>2\<^bold>{p\<^bold>} \<rbrakk> \<Longrightarrow> \<^bold>{p \<and> q\<^bold>}Q\<^sub>1 ;; Q\<^sub>2\<^bold>{p\<^bold>}"
   using seq_hoare_r by blast
     
-lemma seq_hoare_inv_r_2 [hoare]: "\<lbrakk> \<^bold>{p\<^bold>}Q\<^sub>1\<^bold>{q\<^bold>} ; \<^bold>{q\<^bold>}Q\<^sub>2\<^bold>{q\<^bold>} \<rbrakk> \<Longrightarrow> \<^bold>{p\<^bold>}Q\<^sub>1 \<Zcomp> Q\<^sub>2\<^bold>{q\<^bold>}"
+lemma seq_hoare_inv_r_2 [hoare]: "\<lbrakk> \<^bold>{p\<^bold>}Q\<^sub>1\<^bold>{q\<^bold>} ; \<^bold>{q\<^bold>}Q\<^sub>2\<^bold>{q\<^bold>} \<rbrakk> \<Longrightarrow> \<^bold>{p\<^bold>}Q\<^sub>1 ;; Q\<^sub>2\<^bold>{q\<^bold>}"
   using seq_hoare_r by blast
 
-lemma seq_hoare_inv_r_3 [hoare]: "\<lbrakk> \<^bold>{p\<^bold>}Q\<^sub>1\<^bold>{p\<^bold>} ; \<^bold>{p\<^bold>}Q\<^sub>2\<^bold>{q\<^bold>} \<rbrakk> \<Longrightarrow> \<^bold>{p\<^bold>}Q\<^sub>1 \<Zcomp> Q\<^sub>2\<^bold>{q\<^bold>}"
+lemma seq_hoare_inv_r_3 [hoare]: "\<lbrakk> \<^bold>{p\<^bold>}Q\<^sub>1\<^bold>{p\<^bold>} ; \<^bold>{p\<^bold>}Q\<^sub>2\<^bold>{q\<^bold>} \<rbrakk> \<Longrightarrow> \<^bold>{p\<^bold>}Q\<^sub>1 ;; Q\<^sub>2\<^bold>{q\<^bold>}"
   using seq_hoare_r by blast
 
 subsection \<open> Assignment Laws \<close>
 
 lemma assigns_hoare_r [hoare_safe]: "`p \<longrightarrow> \<sigma> \<dagger> q` \<Longrightarrow> \<^bold>{p\<^bold>}\<langle>\<sigma>\<rangle>\<^sub>a\<^bold>{q\<^bold>}"
-  by rel_auto
+  by pred_auto
   
 lemma assigns_backward_hoare_r: 
   "\<^bold>{\<sigma> \<dagger> p\<^bold>}\<langle>\<sigma>\<rangle>\<^sub>a\<^bold>{p\<^bold>}"
-  by rel_auto
+  by pred_auto
 
 lemma assign_floyd_hoare_r:
   assumes "vwb_lens x"
   shows "\<^bold>{p\<^bold>} x := e \<^bold>{\<exists> v . p\<lbrakk>\<guillemotleft>v\<guillemotright>/x\<rbrakk> \<and> $x = e\<lbrakk>\<guillemotleft>v\<guillemotright>/x\<rbrakk>\<^bold>}"
   using assms
-  by (rel_auto, metis lens_override_def lens_override_idem)
+  by (pred_auto, metis lens_override_def lens_override_idem)
 
 lemma assigns_init_hoare [hoare_safe]:
-  "\<lbrakk> vwb_lens x; $x \<sharp> p; $x \<sharp> v; \<^bold>{$x = v \<and> p\<^bold>}S\<^bold>{q\<^bold>} \<rbrakk> \<Longrightarrow> \<^bold>{p\<^bold>}(x := v) \<Zcomp> S\<^bold>{q\<^bold>}"
-  by rel_auto
+  "\<lbrakk> vwb_lens x; $x \<sharp> p; $x \<sharp> v; \<^bold>{$x = v \<and> p\<^bold>}S\<^bold>{q\<^bold>} \<rbrakk> \<Longrightarrow> \<^bold>{p\<^bold>}(x := v) ;; S\<^bold>{q\<^bold>}"
+  by pred_auto
 
 lemma assigns_init_hoare_general:
   "\<lbrakk> vwb_lens x; \<And> x\<^sub>0. \<^bold>{$x = v\<lbrakk>\<guillemotleft>x\<^sub>0\<guillemotright>/x\<rbrakk> \<and> p\<lbrakk>\<guillemotleft>x\<^sub>0\<guillemotright>/x\<rbrakk>\<^bold>}S\<^bold>{q\<^bold>} \<rbrakk> \<Longrightarrow> \<^bold>{p\<^bold>}x := v ;; S\<^bold>{q\<^bold>}"
-  by (rule seq_hoare_r, rule assign_floyd_hoare_r, simp, rel_auto)
+  by (rule seq_hoare_r, rule assign_floyd_hoare_r, simp, pred_auto)
 
 lemma assigns_final_hoare [hoare_safe]:
   "\<^bold>{p\<^bold>}S\<^bold>{\<sigma> \<dagger> q\<^bold>} \<Longrightarrow> \<^bold>{p\<^bold>}S ;; \<langle>\<sigma>\<rangle>\<^sub>a\<^bold>{q\<^bold>}"
-  by (rel_auto)
+  by (pred_auto)
 
 lemma skip_hoare_r [hoare_safe]: "\<^bold>{p\<^bold>}II\<^bold>{p\<^bold>}"
-  by rel_auto
+  by pred_auto
 
 lemma skip_hoare_impl_r [hoare_safe]: "`p \<longrightarrow> q` \<Longrightarrow> \<^bold>{p\<^bold>}II\<^bold>{q\<^bold>}"
-  by rel_auto  
+  by pred_auto  
 
 subsection \<open> Conditional Laws \<close>
 
@@ -145,17 +144,17 @@ lemma cond_hoare_r_sp:
 lemma hoare_ndet [hoare_safe]: 
   assumes "\<^bold>{p\<^bold>}P\<^bold>{q\<^bold>}" "\<^bold>{p\<^bold>}Q\<^bold>{q\<^bold>}"
   shows "\<^bold>{p\<^bold>}(P \<union> Q)\<^bold>{q\<^bold>}"
-  using assms by (rel_auto)
+  using assms by (pred_auto)
 
 lemma hoare_disj [hoare_safe]: 
   assumes "\<^bold>{p\<^bold>}P\<^bold>{q\<^bold>}" "\<^bold>{p\<^bold>}Q\<^bold>{q\<^bold>}"
   shows "\<^bold>{p\<^bold>}(P \<or> Q)\<^bold>{q\<^bold>}"
-  using assms by (rel_auto)
+  using assms by (pred_auto)
 
 lemma hoare_UINF [hoare_safe]:
   assumes "\<And>i. i \<in> A \<Longrightarrow> \<^bold>{p\<^bold>}P(i)\<^bold>{q\<^bold>}"
   shows "\<^bold>{p\<^bold>}(\<Union> {P(i)|i. i\<in>A})\<^bold>{q\<^bold>}"
-  using assms by (rel_auto, meson hoare_meaning)
+  using assms by (pred_auto, meson hoare_meaning)
 
 
 subsection \<open> Recursion Laws \<close>
@@ -163,7 +162,7 @@ subsection \<open> Recursion Laws \<close>
 lemma nu_hoare_r_partial: 
   assumes induct_step: "\<And>P st. \<^bold>{p\<^bold>}P\<^bold>{q\<^bold>} \<Longrightarrow> \<^bold>{p\<^bold>}F P\<^bold>{q\<^bold>}"   
   shows "\<^bold>{p\<^bold>}\<nu> F\<^bold>{q\<^bold>}"
-  using induct_step by (rel_auto add: lfp_lowerbound)
+  using induct_step by (pred_auto add: lfp_lowerbound)
 
 lemma mu_hoare_r:
   assumes WF: "wf R"
@@ -191,15 +190,15 @@ lemma mu_hoare_r':
 subsection \<open> Iteration Rules \<close>
 
 lemma iter_hoare_r [hoare_safe]: "\<^bold>{P\<^bold>}S\<^bold>{P\<^bold>} \<Longrightarrow> \<^bold>{P\<^bold>}S\<^sup>*\<^bold>{P\<^bold>}"
-   using rtrancl_induct by (rel_auto, fastforce)
+   using rtrancl_induct by (pred_auto, fastforce)
 
 lemma while_hoare_r [hoare_safe]:
   assumes "\<^bold>{p \<and> b\<^bold>}S\<^bold>{p\<^bold>}"
   shows "\<^bold>{p\<^bold>}while b do S od\<^bold>{\<not>b \<and> p\<^bold>}"
 proof (simp add: while_top_def hoare_r_def assms)
-  have "(p\<^sup>< \<longrightarrow> (\<not> b \<and> p)\<^sup>>)\<^sub>u \<sqsubseteq> S \<Zcomp> (p\<^sup>< \<longrightarrow> (\<not> b \<and> p)\<^sup>>)\<^sub>u \<^bold>\<lhd> b \<^bold>\<rhd> II"
-    using assms by rel_auto
-  then show "(p\<^sup>< \<longrightarrow> (\<not> b \<and> p)\<^sup>>)\<^sub>u \<sqsubseteq> (\<nu> X \<bullet> S \<Zcomp> X \<^bold>\<lhd> b \<^bold>\<rhd> II)"
+  have "(p\<^sup>< \<longrightarrow> (\<not> b \<and> p)\<^sup>>)\<^sub>u \<sqsubseteq> S ;; (p\<^sup>< \<longrightarrow> (\<not> b \<and> p)\<^sup>>)\<^sub>u \<^bold>\<lhd> b \<^bold>\<rhd> II"
+    using assms by pred_auto
+  then show "(p\<^sup>< \<longrightarrow> (\<not> b \<and> p)\<^sup>>)\<^sub>u \<sqsubseteq> (\<nu> X \<bullet> S ;; X \<^bold>\<lhd> b \<^bold>\<rhd> II)"
     by (simp add: lfp_lowerbound ref_by_set_def)
 qed
 
@@ -216,7 +215,7 @@ lemma while_r_minimal_partial:
 
 (*lemma approx_chain: 
   "(\<Sqinter>n::nat. \<lceil>p \<and> v <\<^sub>u \<guillemotleft>n\<guillemotright>\<rceil>\<^sub><) = \<lceil>p\<rceil>\<^sub><"
-  by (rel_auto)*)
+  by (pred_auto)*)
 
 text \<open> Total correctness law for Hoare logic, based on constructive chains. This is limited to
   variants that have naturals numbers as their range. \<close>
@@ -225,23 +224,23 @@ lemma while_term_hoare_r:
   assumes "\<And> z::nat. \<^bold>{p \<and> b \<and> v = \<guillemotleft>z\<guillemotright>\<^bold>}S\<^bold>{p \<and> v < \<guillemotleft>z\<guillemotright>\<^bold>}"
   shows "\<^bold>{p\<^bold>}while\<^sub>\<bottom> b do S od\<^bold>{\<not>b \<and> p\<^bold>}"
 proof -
-  have "((p\<^sup><)\<^sub>u \<Rightarrow> ((\<not> b \<and> p)\<^sup>>)\<^sub>u) \<sqsubseteq> (\<mu> X \<bullet> S \<Zcomp> X \<^bold>\<lhd> b \<^bold>\<rhd> II)"
+  have "((p\<^sup><)\<^sub>u \<Rightarrow> ((\<not> b \<and> p)\<^sup>>)\<^sub>u) \<sqsubseteq> (\<mu> X \<bullet> S ;; X \<^bold>\<lhd> b \<^bold>\<rhd> II)"
   proof (rule mu_refine_intro)
-    from assms show "((p\<^sup><)\<^sub>u \<Rightarrow> ((\<not> b \<and> p)\<^sup>>)\<^sub>u) \<sqsubseteq> S \<Zcomp> ((p\<^sup><)\<^sub>u \<Rightarrow> ((\<not> b \<and> p)\<^sup>>)\<^sub>u) \<^bold>\<lhd> b \<^bold>\<rhd> II"
-      by (rel_auto; smt (z3) hoare_meaning)+
+    from assms show "((p\<^sup><)\<^sub>u \<Rightarrow> ((\<not> b \<and> p)\<^sup>>)\<^sub>u) \<sqsubseteq> S ;; ((p\<^sup><)\<^sub>u \<Rightarrow> ((\<not> b \<and> p)\<^sup>>)\<^sub>u) \<^bold>\<lhd> b \<^bold>\<rhd> II"
+      by (pred_auto; smt (z3) hoare_meaning)+
     let ?E = "\<lambda> n. \<lbrakk>(p \<and> v < \<guillemotleft>n\<guillemotright>)\<^sup><\<rbrakk>\<^sub>u"
-    show "((p\<^sup><)\<^sub>u \<and> (\<mu> X \<bullet> S \<Zcomp> X \<^bold>\<lhd> b \<^bold>\<rhd> II)) = ((p\<^sup><)\<^sub>u \<and> (\<nu> X \<bullet> S \<Zcomp> X \<^bold>\<lhd> b \<^bold>\<rhd> II))"
+    show "((p\<^sup><)\<^sub>u \<and> (\<mu> X \<bullet> S ;; X \<^bold>\<lhd> b \<^bold>\<rhd> II)) = ((p\<^sup><)\<^sub>u \<and> (\<nu> X \<bullet> S ;; X \<^bold>\<lhd> b \<^bold>\<rhd> II))"
     proof (rule constr_fp_uniq[where E="?E"])
-      show "mono (\<lambda>X. S \<Zcomp> X \<^bold>\<lhd> b \<^bold>\<rhd> II)"
+      show "mono (\<lambda>X. S ;; X \<^bold>\<lhd> b \<^bold>\<rhd> II)"
         by (rule cond_seqr_mono)
-      show "constr (\<lambda>X. S \<Zcomp> X \<^bold>\<lhd> b \<^bold>\<rhd> II) ?E"
+      show "constr (\<lambda>X. S ;; X \<^bold>\<lhd> b \<^bold>\<rhd> II) ?E"
         apply (rule constrI, rule chainI)
-          apply (rel_auto)+
+          apply (pred_auto)+
         by (smt (verit, del_insts) assms hoare_meaning less_Suc_eq order_less_trans)+
-    qed rel_auto (* Couldn't pattern match last goal *)
+    qed pred_auto (* Couldn't pattern match last goal *)
   qed
   thus ?thesis
-    by (rel_auto add: while_bot_def)
+    by (pred_auto add: while_bot_def)
 qed
 
 lemma while_vrt_hoare_r [hoare_safe]:
@@ -266,15 +265,15 @@ proof (rule pre_weak_rel[of _ "p\<^sup><" ], goal_cases)
   from I0 show ?case by expr_auto
 next
   case 2
-  have "(p\<^sup>< \<longrightarrow> q'\<^sup>>)\<^sub>u \<sqsubseteq> (\<mu> X \<bullet> Q \<Zcomp> X \<^bold>\<lhd> b \<^bold>\<rhd> II)"
+  have "(p\<^sup>< \<longrightarrow> q'\<^sup>>)\<^sub>u \<sqsubseteq> (\<mu> X \<bullet> Q ;; X \<^bold>\<lhd> b \<^bold>\<rhd> II)"
   proof (rule mu_rec_total_utp_rule[where e=e, OF WF])
-    show "mono (\<lambda>X. Q \<Zcomp> X \<^bold>\<lhd> b \<^bold>\<rhd> II)"
+    show "mono (\<lambda>X. Q ;; X \<^bold>\<lhd> b \<^bold>\<rhd> II)"
       by (simp add: cond_seqr_mono)
     have induct_step': "\<And> st. ((b \<and> p \<and> e = \<guillemotleft>st\<guillemotright>)\<^sup>< \<longrightarrow> (p \<and> (e,\<guillemotleft>st\<guillemotright>) \<in> \<guillemotleft>R\<guillemotright>)\<^sup>>)\<^sub>u \<sqsubseteq> Q"
-      using induct_step by rel_auto  
+      using induct_step by pred_auto  
     with PHI
-    show "\<And>st. (p\<^sup>< \<and> e\<^sup>< = \<guillemotleft>st\<guillemotright> \<longrightarrow> q'\<^sup>>)\<^sub>u \<sqsubseteq> Q \<Zcomp> (p\<^sup>< \<and> (e\<^sup><, \<guillemotleft>st\<guillemotright>) \<in> \<guillemotleft>R\<guillemotright> \<longrightarrow> q'\<^sup>>)\<^sub>u \<^bold>\<lhd> b \<^bold>\<rhd> II"
-      apply rel_auto
+    show "\<And>st. (p\<^sup>< \<and> e\<^sup>< = \<guillemotleft>st\<guillemotright> \<longrightarrow> q'\<^sup>>)\<^sub>u \<sqsubseteq> Q ;; (p\<^sup>< \<and> (e\<^sup><, \<guillemotleft>st\<guillemotright>) \<in> \<guillemotleft>R\<guillemotright> \<longrightarrow> q'\<^sup>>)\<^sub>u \<^bold>\<lhd> b \<^bold>\<rhd> II"
+      apply pred_auto
       by (smt (z3) hoare_meaning induct_step)+
   qed
   then show ?case by simp
@@ -293,35 +292,35 @@ lemma frame_hoare_r:
   assumes "idem_scene a" "a \<sharp> r" "-a \<sharp> q" "\<^bold>{p\<^bold>}P\<^bold>{q\<^bold>}"
   shows "\<^bold>{p \<and> r\<^bold>}a:[P]\<^bold>{q \<and> r\<^bold>}"
   using assms
-  apply (rel_auto)
+  apply (pred_auto)
    apply (metis (mono_tags, lifting) Product_Type.Collect_case_prodD frame_def fst_conv hoare_meaning snd_conv)
   by (metis (mono_tags, lifting) Product_Type.Collect_case_prodD frame_def fst_eqD scene_equiv_def scene_override_commute snd_eqD)
 
 lemma frame_strong_hoare_r [hoare_safe]: 
   assumes "idem_scene a" "a \<sharp> r" "-a \<sharp> q" "\<^bold>{p \<and> r\<^bold>}S\<^bold>{q\<^bold>}"
   shows "\<^bold>{p \<and> r\<^bold>}a:[S]\<^bold>{q \<and> r\<^bold>}"
-  using assms apply (rel_auto)
+  using assms apply (pred_auto)
    apply (metis (mono_tags, lifting) SEXP_def hoare_meaning rel_frame set_pred_def)
   by (metis SEXP_def rel_frame scene_equiv_def scene_override_commute set_pred_def)
 
 lemma frame_hoare_r' [hoare_safe]: 
   assumes "idem_scene a" "a \<sharp> r" "-a \<sharp> q" "\<^bold>{r \<and> p\<^bold>}S\<^bold>{q\<^bold>}"
   shows "\<^bold>{r \<and> p\<^bold>}a:[S]\<^bold>{r \<and> q\<^bold>}"
-  using assms apply (rel_auto)
+  using assms apply (pred_auto)
    apply (metis SEXP_def rel_frame scene_equiv_def scene_override_commute set_pred_def)
   by (metis (mono_tags, lifting) Product_Type.Collect_case_prodD frame_def fst_conv hoare_meaning snd_conv)
 
 lemma antiframe_hoare_r:
   assumes "idem_scene a" "-a \<sharp> r" "a \<sharp> q" "\<^bold>{p\<^bold>}P\<^bold>{q\<^bold>}"  
   shows "\<^bold>{p \<and> r\<^bold>} (-a):[P] \<^bold>{q \<and> r\<^bold>}"
-  using assms apply (rel_auto)
+  using assms apply (pred_auto)
    apply (metis (mono_tags, lifting) Product_Type.Collect_case_prodD frame_def fst_conv hoare_meaning snd_conv)
   by (metis (full_types) SEXP_def rel_frame scene_equiv_def scene_override_commute set_pred_def)
     
 lemma antiframe_strong_hoare_r:
   assumes "idem_scene a" "-a \<sharp> r" "a \<sharp> q" "\<^bold>{p \<and> r\<^bold>}P\<^bold>{q\<^bold>}"  
   shows "\<^bold>{p \<and> r\<^bold>} (-a):[P] \<^bold>{q \<and> r\<^bold>}"
-  using assms  apply (rel_auto)
+  using assms  apply (pred_auto)
    apply (metis (mono_tags, lifting) Product_Type.Collect_case_prodD frame_def fst_conv hoare_meaning snd_conv)
   by (metis (full_types) SEXP_def rel_frame scene_equiv_def scene_override_commute set_pred_def)
 
@@ -329,15 +328,15 @@ lemma antiframe_strong_hoare_r:
 lemma nmods_invariant:
   assumes "S nmods a" "-a \<sharp> p"
   shows "\<^bold>{p\<^bold>}S\<^bold>{p\<^bold>}"
-  using assms apply rel_auto
+  using assms apply pred_auto
   by (metis Healthy_def SEXP_def rel_frame scene_equiv_def scene_override_commute set_pred_def)
 
 (*
 lemma hoare_r_ghost:
-  assumes "vwb_lens x" "x \<sharp> p" "x \<sharp> q" "S nuses x" "\<^bold>{p\<^bold>}x := e\<Zcomp> S\<^bold>{q\<^bold>}"
+  assumes "vwb_lens x" "x \<sharp> p" "x \<sharp> q" "S nuses x" "\<^bold>{p\<^bold>}x := e;; S\<^bold>{q\<^bold>}"
   shows "\<^bold>{p\<^bold>}S\<^bold>{q\<^bold>}" 
 proof -
-  have "\<^bold>{p\<^bold>}x := e\<Zcomp> rrestr x S\<^bold>{q\<^bold>}"
+  have "\<^bold>{p\<^bold>}x := e;; rrestr x S\<^bold>{q\<^bold>}"
     by (simp add: Healthy_if assms(4) assms(5))
   with assms(1-3) have "\<^bold>{p\<^bold>}rrestr x S\<^bold>{q\<^bold>}"
     by (rel_simp,metis mwb_lens.put_put vwb_lens_mwb)
